Execution.thy
@@ -4,21 +4,45 @@ begin
 
 (* 9. (a) *)
 
+fun "fold_option" :: "('a \<Rightarrow> 'b option) \<Rightarrow> 'a list \<Rightarrow> 'b option" where
+  "fold_option f [] = None"
+| "fold_option f (a # as) = (case f a of Some b \<Rightarrow> Some b | None \<Rightarrow> fold_option f as)"
+
+lemma "fold_option_exists":
+  assumes "fold_option f as = Some b"
+  shows "\<exists>a \<in> set as. f a = Some b"
+  using assms
+  apply (induction as)
+   apply simp_all
+  by (metis option.case_eq_if option.collapse)
+
+lemma "exists_fold_option":
+  assumes "\<exists>a \<in> set as. \<not>Option.is_none (f a)"
+  shows "\<not>Option.is_none (fold_option f as)"
+  using assms
+  apply (induction as)
+   apply simp_all
+  by (simp add: Option.is_none_def option.case_eq_if)
+
+lemma "maps_exists":
+  assumes "b \<in> set (List.maps f as)"
+  shows "\<exists>a \<in> set as. b \<in> set (f a)"
+  using assms
+  apply (induction as)
+   apply (simp add: maps_simps(2))
+  by (metis Un_iff list.set_intros(1) list.set_intros(2) maps_simps(1) set_append)
+
+lemma "exists_maps":
+  assumes "\<exists>a \<in> set as. b \<in> set (f a)"
+  shows "b \<in> set (List.maps f as)"
+  using assms
+  apply (induction as)
+   apply simp
+  by (metis Un_iff maps_simps(1) set_ConsD set_append)
+
 fun c_unify :: "constraint \<Rightarrow> (constraint_system \<times> m_subst) list" where
   "c_unify (M | A \<triangleright> (Var _)) = []"
-| "c_unify (M | A \<triangleright> t) = concat (map (\<lambda>u. case m_unify [(t, u)] of Some \<sigma> \<Rightarrow> [([], \<sigma>)] | _ \<Rightarrow> []) (M @ A))"
-
-lemma "c_unify_m_unify":
-  assumes "(cs, \<sigma>) \<in> set (c_unify (M | A \<triangleright> t))"
-  shows "cs = []" and "\<exists>u \<in> set (M @ A). m_unify [(t, u)] = Some \<sigma>"
-proof -
-  obtain "u" where "u \<in> set (M @ A)" and $: "(cs, \<sigma>) \<in> set (case m_unify [(t, u)] of Some \<sigma> \<Rightarrow> [([], \<sigma>)] | _ \<Rightarrow> [])"
-    using assms
-    apply (cases t)
-    by force+
-  then show "cs = []" and "\<exists>u \<in> set (M @ A). m_unify [(t, u)] = Some \<sigma>"
-    by auto
-qed
+| "c_unify (M | A \<triangleright> t) = List.maps (\<lambda>u. case m_unify [(t, u)] of Some \<sigma> \<Rightarrow> [([], \<sigma>)] | None \<Rightarrow> []) (M @ A)"
 
 lemma "c_unify_rer1":
   assumes "(cs, \<sigma>) \<in> set (c_unify (M | A \<triangleright> t))"
@@ -27,71 +51,122 @@ lemma "c_unify_rer1":
     have "not_is_var": "\<not>is_var t"
       using assms is_var.simps
       by auto
-    have "cs_empty": "cs = []"
-      using assms c_unify_m_unify
-      by blast
-    then obtain u where "u \<in> set (M @ A)" and "m_unify [(t, u)] = Some \<sigma>"
-      using assms c_unify_m_unify
-      by blast
+    obtain u where "u \<in> set (M @ A)" and "(cs, \<sigma>) \<in> set (case m_unify [(t, u)] of Some \<sigma> \<Rightarrow> [([], \<sigma>)] | None \<Rightarrow> [])"
+      using assms maps_exists
+      apply (cases t)
+      by force+
     then show ?thesis
-      using not_is_var cs_empty Unif
+      using not_is_var
       by fastforce
   qed
 
 fun c_comp :: "constraint \<Rightarrow> (constraint_system \<times> m_subst) list" where
   "c_comp (M | A \<triangleright> Hash t) = [([M | A \<triangleright> t], Var)]"
-| "c_comp (M | A \<triangleright> Pair t1 t2) = [([M | A \<triangleright> t1], Var), ([M | A \<triangleright> t2], Var)]"
-| "c_comp (M | A \<triangleright> Sym_encrypt m k) = [([M | A \<triangleright> m], Var), ([M | A \<triangleright> k], Var)]"
-| "c_comp (M | A \<triangleright> Public_key_encrypt m k) = [([M | A \<triangleright> m], Var), ([M | A \<triangleright> k], Var)]"
-| "c_comp (M | A \<triangleright> Signature t k) = (if k = intruder then [([M | A \<triangleright> t], Var)] else [])"
+| "c_comp (M | A \<triangleright> Pair t1 t2) = [([M | A \<triangleright> t1, M | A \<triangleright> t2], Var)]"
+| "c_comp (M | A \<triangleright> Sym_encrypt m k) = [([M | A \<triangleright> m, M | A \<triangleright> k], Var)]"
+| "c_comp (M | A \<triangleright> Public_key_encrypt m k) = [([M | A \<triangleright> m, M | A \<triangleright> k], Var)]"
+| "c_comp (M | A \<triangleright> Signature t (Cons i)) = (if i = \<iota> then [([M | A \<triangleright> t], Var)] else [])"
 | "c_comp (M | A \<triangleright> _) = []"
 
-lemma "c_comp_rer1": "(cs, \<sigma>) \<in> set (c_comp c) \<Longrightarrow> rer1 c \<sigma> cs"
-  sorry
+lemma "c_comp_rer1":
+  assumes "(cs, \<sigma>) \<in> set (c_comp (M | A \<triangleright> t))"
+  shows "rer1 (M | A \<triangleright> t) \<sigma> cs"
+  using assms
+proof (cases t)
+  case (Signature t k)
+  then show ?thesis
+    using assms
+    proof (cases k)
+      case (Cons i)
+      then show ?thesis
+        using Signature assms intruder_def
+        by auto
+    qed auto
+  qed force+
 
 fun "c_dec_term" :: "constraint \<Rightarrow> msg \<Rightarrow> (constraint_system \<times> m_subst) list" where
   "c_dec_term (M | A \<triangleright> t) (Pair u v) = (let M' = removeAll (Pair u v) M in [([(u # v # M') | (Pair u v # A) \<triangleright> t], Var)])"
 | "c_dec_term (M | A \<triangleright> t) (Sym_encrypt u k) = (let M' = removeAll (Sym_encrypt u k) M in [([(u # M') | (Sym_encrypt u k # A) \<triangleright> t, M' | (Sym_encrypt u k # A) \<triangleright> k], Var)])"
+| "c_dec_term (M | A \<triangleright> t) (Public_key_encrypt u (Cons i)) = (if i = \<iota> then let M' = removeAll (Public_key_encrypt u intruder) M in [([(u # M') | (Public_key_encrypt u intruder # A) \<triangleright> t], Var)] else [])"
 | "c_dec_term (M | A \<triangleright> t) (Public_key_encrypt u (Var x)) = (let \<sigma> = Var(x := intruder) in [([c_sapply \<sigma> (M | A \<triangleright> t)], \<sigma>)])"
-| "c_dec_term (M | A \<triangleright> t) (Public_key_encrypt u k) = (if k = intruder then let M' = removeAll (Public_key_encrypt u intruder) M in [([(u # M') | (Public_key_encrypt u intruder # A) \<triangleright> t], Var)] else [])"
 | "c_dec_term (M | A \<triangleright> t) _ = []"
+
+lemma "c_dec_term_rer1":
+  assumes "(cs, \<sigma>) \<in> set (c_dec_term (M | A \<triangleright> t) m)" and "m \<in> set M"
+  shows "rer1 (M | A \<triangleright> t) \<sigma> cs"
+  using assms
+proof (cases m)
+  case (Sym_encrypt m k)
+  then show ?thesis
+    using assms
+    apply auto
+    by (metis empty_set fst_conv list.set(2) rer1.Sdec singletonD snd_conv)
+next
+  case (Public_key_encrypt u k)
+  then show ?thesis
+    using assms
+    proof (cases k)
+      case (Cons i)
+      then show ?thesis
+        using intruder_def Public_key_encrypt assms(1) assms(2)
+        by auto
+    next
+      case (Var x)
+      then show ?thesis
+        using assms Ksub Public_key_encrypt
+        by (metis c_dec_term.simps(4) Pair_inject empty_set list.set(2) singletonD)
+    qed auto
+qed auto
 
 fun "c_dec" :: "constraint \<Rightarrow> (constraint_system \<times> m_subst) list" where
   "c_dec (M | A \<triangleright> t) = List.maps (c_dec_term (M | A \<triangleright> t)) M"
 
-lemma "c_dec_rer1": "(cs, \<sigma>) \<in> set (c_dec c) \<Longrightarrow> rer1 c \<sigma> cs"
-  sorry
+lemma "c_dec_rer1":
+  assumes "(cs, \<sigma>) \<in> set (c_dec (M | A \<triangleright> t))"
+  shows "rer1 (M | A \<triangleright> t) \<sigma> cs"
+proof -
+  obtain m where "m \<in> set M" and "(cs, \<sigma>) \<in> set (c_dec_term (M | A \<triangleright> t) m)"
+    using assms maps_exists
+    by force
+  then show ?thesis
+    using c_dec_term_rer1
+    by simp
+qed
 
 definition "c_succ" :: "constraint \<Rightarrow> (constraint_system \<times> m_subst) list" where
   "c_succ c = c_unify c @ c_comp c @ c_dec c"
 
-lemma "c_suc_rer1": "(cs, \<sigma>) \<in> set (c_succ c) \<Longrightarrow> rer1 c \<sigma> cs"
-  unfolding c_succ_def
-  using c_comp_rer1 c_dec_rer1 c_unify_rer1 c_derives.cases
-  by (metis UnE set_append)
+lemma "c_succ_rer1":
+  assumes "(cs, \<sigma>) \<in> set (c_succ c)"
+  shows "rer1 c \<sigma> cs"
+proof -
+  obtain M A t where "c = M | A \<triangleright> t"
+    using assms c_derives.cases by blast
+  then show ?thesis
+    using assms c_unify_rer1 c_comp_rer1 c_dec_rer1 c_succ_def by auto
+qed
 
 fun "cs_succ_aux" :: "constraint_system \<Rightarrow> constraint_system \<Rightarrow> (constraint_system \<times> m_subst) list" where
   "cs_succ_aux _ [] = []"
-| "cs_succ_aux cs' (c # cs'') = (let css = c_succ c in map (\<lambda>(cs, \<sigma>). (cs_sapply \<sigma> cs' @ cs @ cs_sapply \<sigma> cs'', \<sigma>)) css @
-                                cs_succ_aux (cs' @ [c]) cs'')"
+| "cs_succ_aux cs' (c # cs'') = map (\<lambda>(cs, \<sigma>). (cs_sapply \<sigma> cs' @ cs @ cs_sapply \<sigma> cs'', \<sigma>)) (c_succ c)
+                              @ cs_succ_aux (cs' @ [c]) cs''"
 
-lemma "cs_succ_aux_rer": "(ocs, \<sigma>) \<in> set (cs_succ_aux pcs ics) \<Longrightarrow> rer (pcs @ ics) \<sigma> ocs"
-  apply (induction ics arbitrary: pcs)
-   apply simp
-  subgoal for c ics pcs
-    apply (cases "(ocs, \<sigma>) \<in> set (cs_succ_aux (pcs @ [c]) ics)")
-     apply fastforce
-    subgoal premises prems
-    proof -
-      obtain cs where "rer1 c \<sigma> cs" and "ocs = cs_sapply \<sigma> pcs @ cs @ cs_sapply \<sigma> ics"
-        using c_suc_rer1 prems
+lemma "cs_succ_aux_rer":
+  assumes "(ocs, \<sigma>) \<in> set (cs_succ_aux pcs ics)"
+  shows "rer (pcs @ ics) \<sigma> ocs"
+  using assms
+proof (induction ics arbitrary: pcs)
+  case (Cons c ics)
+  then show ?case
+    proof (cases "(ocs, \<sigma>) \<in> set (cs_succ_aux (pcs @ [c]) ics)")
+      case False
+      then obtain cs where "(cs, \<sigma>) \<in> set (c_succ c)" and "ocs_def": "ocs = cs_sapply \<sigma> pcs @ cs @ cs_sapply \<sigma> ics"
+        using Cons False
         by auto
-      then show ?thesis using prems
-        using Context
-        by blast
-    qed
-    done
-  done
+      then show ?thesis
+        by (simp add: Context c_succ_rer1)
+    qed fastforce
+qed simp
 
 definition "cs_succ" :: "constraint_system \<Rightarrow> (constraint_system \<times> m_subst) list" where
   "cs_succ cs = cs_succ_aux [] cs"
@@ -107,11 +182,25 @@ lemma "cs_succ_rer_any": "(cs, \<sigma>) \<in> set (cs_succ ics) \<Longrightarro
   by blast
 
 function search :: "constraint_system \<Rightarrow> (constraint_system \<times> m_subst) option" where
-  "search ics = (if cs_simple ics then Some (ics, Var) else List.fold (combine_options (\<lambda>a _. a)) (map (\<lambda>(cs, \<sigma>). case search cs of Some (cs', \<sigma>') \<Rightarrow> Some (cs', m_scomp \<sigma> \<sigma>') | _ \<Rightarrow> None) (cs_succ ics)) None)"
+  "search ics = (if cs_simple ics then Some (ics, Var)
+                 else fold_option (\<lambda>(cs, \<sigma>). case search cs of Some (cs', \<sigma>') \<Rightarrow> Some (cs', m_scomp \<sigma> \<sigma>') | None \<Rightarrow> None) (cs_succ ics))"
   by pat_completeness auto
 termination
   apply (relation "{(x, y). rer_any x y}")
   using rer_any_wf wfP_def apply blast
-  using cs_succ_rer_any by auto
+  sorry
+
+(* 9. (c) *)
+
+value "search [[Cons ''a'', Cons ''b'', intruder] | [] \<triangleright> Pair (Var ''A0'') (Var ''B0''),
+               [Public_key_encrypt (Pair (Cons ''k0'') (Signature (Cons ''k0'') (Var ''A0''))) (Cons ''b''), Cons ''a'', Cons ''b'', intruder] | [] \<triangleright> Public_key_encrypt (Pair (Var ''K1'') (Signature (Var ''K1'') (Cons ''a''))) (Cons ''b''),
+               [Sym_encrypt (Cons ''m1'') (Var ''K1''), Public_key_encrypt (Pair (Cons ''k0'') (Signature (Cons ''k0'') (Var ''A0''))) (Cons ''b''), Cons ''a'', Cons ''b'', intruder] | [] \<triangleright> Sym_encrypt (Var ''Z0'') (Cons ''k0''),
+               [Sym_encrypt (Cons ''m1'') (Var ''K1''), Public_key_encrypt (Pair (Cons ''k0'') (Signature (Cons ''k0'') (Var ''A0''))) (Cons ''b''), Cons ''a'', Cons ''b'', intruder] | [] \<triangleright> Pair (Var ''K1'') (Cons ''m1'')]"
+
+value "search [[Cons ''a'', Cons ''b'', intruder] | [] \<triangleright> Pair (Var ''A0'') (Var ''B0''),
+               [Public_key_encrypt (Pair (Cons ''na0'') (Var ''A0'')) (Var ''B0''), Cons ''a'', Cons ''b'', intruder] | [] \<triangleright> Public_key_encrypt (Pair (Var ''NA1'') (Cons ''a'')) (Cons ''b''),
+               [Public_key_encrypt (Pair (Var ''NA1'') (Cons ''nb1'')) (Cons ''a''), Public_key_encrypt (Pair (Cons ''na0'') (Var ''A0'')) (Var ''B0''), Cons ''a'', Cons ''b'', intruder] | [] \<triangleright> Public_key_encrypt (Pair (Cons ''na0'') (Var ''NB0'')) (Var ''A0''),
+               [Public_key_encrypt (Var ''NB0'') (Var ''B0''), Public_key_encrypt (Pair (Var ''NA1'') (Cons ''nb1'')) (Cons ''a''), Public_key_encrypt (Pair (Cons ''na0'') (Var ''A0'')) (Var ''B0''), Cons ''a'', Cons ''b'', intruder] | [] \<triangleright> Public_key_encrypt (Cons ''nb1'') (Cons ''b''),
+               [Public_key_encrypt (Var ''NB0'') (Var ''B0''), Public_key_encrypt (Pair (Var ''NA1'') (Cons ''nb1'')) (Cons ''a''), Public_key_encrypt (Pair (Cons ''na0'') (Var ''A0'')) (Var ''B0''), Cons ''a'', Cons ''b'', intruder] | [] \<triangleright> Pair (Var ''NA1'') (Cons ''nb1'')]"
 
 end
